{
 "cells": [
  {
   "cell_type": "code",
   "execution_count": null,
   "id": "cc924794-9b76-491d-9b52-781d6fb316bc",
   "metadata": {},
   "outputs": [],
   "source": [
    "( T(2) ) for the recurrence relation ( T(n) = 3T(n-1) + 12n ) with the initial condition ( T(0) = 5 ), we can recursively apply the relation until we reach the desired value.\n",
    "\n",
    "Given that ( T(0) = 5 ), we can compute ( T(1) ) using the recurrence relation:\n",
    "\n",
    "[\n",
    "T(1) = 3T(0) + 12 \\times 1 = 3 times 5 + 12 = 15 + 12 = 27\n",
    "]\n",
    "\n",
    "Now, we can use ( T(1) ) to find ( T(2) ):\n",
    "\n",
    "[\n",
    "T(2) = 3T(1) + 12 \\times 2 = 3 \\times 27 + 12 \\times 2 = 81 + 24 = 105\n",
    "]\n",
    "\n",
    "So, the value of ( T(2) ) is ( 105 )."
   ]
  },
  {
   "cell_type": "code",
   "execution_count": null,
   "id": "750cfb75-f521-4137-8045-7c927340cd66",
   "metadata": {},
   "outputs": [],
   "source": [
    "Sure, let's solve each of these recurrence relations using the substitution method:\n",
    "\n",
    "### a. \\( T(n) = T(n-1) + c \\)\n",
    "\n",
    "To solve this recurrence relation, we'll repeatedly substitute \\( T(n-1) \\), \\( T(n-2) \\), and so on until we reach the base case.\n",
    "\n",
    "Let's start with the base case:\n",
    "\n",
    "- \\( T(1) = T(0) + c \\)\n",
    "- \\( T(2) = T(1) + c = (T(0) + c) + c = T(0) + 2c \\)\n",
    "- \\( T(3) = T(2) + c = (T(0) + 2c) + c = T(0) + 3c \\)\n",
    "\n",
    "From this, we can see a pattern:\n",
    "\n",
    "- \\( T(n) = T(0) + nc \\)\n",
    "\n",
    "So, the solution to the recurrence relation \\( T(n) = T(n-1) + c \\) is \\( T(n) = T(0) + nc \\).\n",
    "\n",
    "### b. \\( T(n) = 2T(n/2) + n \\)\n",
    "\n",
    "This is the recurrence relation for the time complexity of algorithms like Merge Sort.\n",
    "\n",
    "We can guess the solution \\( T(n) = O(n \\log n) \\) and then prove it using the substitution method.\n",
    "\n",
    "Let's assume \\( T(k) = ck\\log k \\) for some constant \\( c \\).\n",
    "\n",
    "Substitute this into the recurrence relation:\n",
    "\n",
    "\\[ T(n) = 2T(n/2) + n \\]\n",
    "\n",
    "\\[ = 2(c(n/2)\\log(n/2)) + n \\]\n",
    "\n",
    "\\[ = cn\\log(n/2) + n \\]\n",
    "\n",
    "\\[ = cn\\log n - cn\\log 2 + n \\]\n",
    "\n",
    "\\[ = cn\\log n - cn + n \\]\n",
    "\n",
    "Now, we need to prove that \\( T(n) \\) is \\( O(n \\log n) \\) by showing \\( T(n) \\leq cn\\log n \\) for some \\( c > 0 \\) and \\( n \\) sufficiently large.\n",
    "\n",
    "Let's choose \\( c \\) such that \\( c \\geq 1 \\) and \\( T(1) \\leq c \\).\n",
    "\n",
    "- \\( T(1) = c \\cdot 1 \\cdot \\log 1 = c \\cdot 0 = 0 \\leq c \\) (True for \\( c \\geq 0 \\))\n",
    "\n",
    "For simplicity, let's ignore the base cases and proceed with the induction step:\n",
    "\n",
    "\\[ T(n) \\leq cn\\log n \\]\n",
    "\n",
    "\\[ 2T(n/2) + n \\leq 2c(n/2)\\log(n/2) + n \\]\n",
    "\\[ = cn\\log(n/2) + n \\]\n",
    "\\[ = cn\\log n - cn\\log 2 + n \\]\n",
    "\\[ = cn\\log n - cn + n \\]\n",
    "\\[ \\leq cn\\log n \\] (For \\( c \\geq 1 \\) and \\( n \\) sufficiently large)\n",
    "\n",
    "Therefore, by induction, we have proven that \\( T(n) \\) is \\( O(n \\log n) \\).\n",
    "\n",
    "### c. \\( T(n) = 2T(n/2) + c \\)\n",
    "\n",
    "This recurrence relation is similar to the one in part b, but the constant term is \\( c \\).\n",
    "\n",
    "Let's assume \\( T(k) = ck\\log k + d \\) for some constants \\( c \\) and \\( d \\).\n",
    "\n",
    "Substitute this into the recurrence relation:\n",
    "\n",
    "\\[ T(n) = 2T(n/2) + c \\]\n",
    "\n",
    "\\[ = 2(c(n/2)\\log(n/2) + d) + c \\]\n",
    "\n",
    "\\[ = cn\\log(n/2) + 2d + c \\]\n",
    "\n",
    "\\[ = cn(\\log n - \\log 2) + 2d + c \\]\n",
    "\n",
    "\\[ = cn\\log n - cn\\log 2 + 2d + c \\]\n",
    "\n",
    "\\[ = cn\\log n - cn + 2d + c \\]\n",
    "\n",
    "Now, we need to prove that \\( T(n) \\) is \\( O(n \\log n) \\) by showing \\( T(n) \\leq cn\\log n \\) for some \\( c > 0 \\) and \\( n \\) sufficiently large.\n",
    "\n",
    "Let's choose \\( c \\) such that \\( c \\geq 1 \\) and \\( T(1) \\leq c \\).\n",
    "\n",
    "- \\( T(1) = c \\cdot 1 \\cdot \\log 1 + d = c \\cdot 0 + d = d \\leq c \\) (True for \\( c \\geq d \\))\n",
    "\n",
    "For simplicity, let's ignore the base cases and proceed with the induction step:\n",
    "\n",
    "\\[ T(n) \\leq cn\\log n \\]\n",
    "\n",
    "\\[ 2T(n/2) + c \\leq 2(c(n/2)\\log(n/2) + d) + c \\]\n",
    "\\[ = cn\\log(n/2) + 2d + c \\]\n",
    "\\[ = cn(\\log n - \\log 2) + 2d + c \\]\n",
    "\\[ = cn\\log n - cn\\log 2 + 2d + c \\]\n",
    "\\[ = cn\\log n - cn + 2d + c \\]\n",
    "\\[ \\leq cn\\log n \\] (For \\( c \\geq 1 \\) and \\( n \\) sufficiently large)\n",
    "\n",
    "Therefore, by induction, we have proven that \\( T(n) \\) is \\( O(n \\log n) \\).\n",
    "\n",
    "### d. \\( T(n) = T(n/2) + c \\)\n",
    "\n",
    "This recurrence relation describes the time complexity of algorithms like Binary Search.\n",
    "\n",
    "Let's solve this relation using the substitution method.\n",
    "\n",
    "Let's assume \\( T(k) = c\\log k \\) for some constant \\( c \\).\n",
    "\n",
    "Substitute this into the recurrence relation:\n",
    "\n",
    "\\[ T(n) = T(n/2) + c \\]\n",
    "\n",
    "\\[ = c\\log(n/2) + c \\]\n",
    "\n",
    "\\[ = c(\\log n - \\log 2) + c \\]\n",
    "\n",
    "\\[ = c\\log n - c\\log 2 + c \\]\n",
    "\n",
    "\\[ = c\\log n - c + c \\]\n",
    "\n",
    "\\[ = c\\log n \\]\n",
    "\n",
    "So, the solution to the recurrence relation \\( T(n) = T(n/2) + c \\) is \\( T(n) = c\\log n \\).\n",
    "\n",
    "This is the time complexity of algorithms like Binary Search, which is \\( O(\\log n) \\)."
   ]
  },
  {
   "cell_type": "code",
   "execution_count": null,
   "id": "bb67a640-6d31-42ee-b866-fa706c9e4c7c",
   "metadata": {},
   "outputs": [],
   "source": [
    "                   T(n)\n",
    "                 /      \\\n",
    "             T(n-1)   T(n-1)\n",
    "            /    \\     /    \\\n",
    "        T(n-2) T(n-2) T(n-2) T(n-2)\n",
    "         /  \\   /   \\  /  \\   /   \\\n",
    "      ...   ...   ...  ...   ...   ...\n",
    "\n",
    "        \n",
    "        \n",
    "        \n",
    "        "
   ]
  }
 ],
 "metadata": {
  "kernelspec": {
   "display_name": "Python 3 (ipykernel)",
   "language": "python",
   "name": "python3"
  },
  "language_info": {
   "codemirror_mode": {
    "name": "ipython",
    "version": 3
   },
   "file_extension": ".py",
   "mimetype": "text/x-python",
   "name": "python",
   "nbconvert_exporter": "python",
   "pygments_lexer": "ipython3",
   "version": "3.10.8"
  }
 },
 "nbformat": 4,
 "nbformat_minor": 5
}
